chore(KSA-Model): more Mutation Operation changes
Explicitly:
- Change InitializeMutationFlag from a union to an enum for ToString reasons
- Model `DoNotVersion` flag for Initialize Mutation
- Refactor Describe Mutation output to detail Input so resume can be done
- Refactor System Key to be optional, detailing that TrustStorage is the default
- More errors
- Smithy changes from PR feedback on #854
- Correction of spelling mistakes
- Mutation Token's UUID is required

Why change the flag to an enum?

Dafny/Smithy-Dafny's support for Union's results in structures that do not print well.
The intention of the  `InitializeMutationFlag` is to inform customers
about the result of their request.

Such information may,
possibly even should,
be logged.

Initialize Mutation and Apply Mutation MUST
ensure that the UUID of the Index and Commitment agree.
Apply MUST ensure that the UUID of the Commitment and Token agree.
The Mutation Token's UUID is REQUIRED.
It is how we track a mutation,
much like how CFN tracks a change set.

Fixed bug where UUID is a reserved word in DDB.

Refactored some of the error messages.
Utilize Java Example to demonstrate resume and restart.
Finally, addressed some of the feedback on PR #854.

AwsCryptographicMaterialProviders/runtimes/java/src/examples/java/software/amazon/cryptography/example/hierarchy/VersionKeyExample.java
@@ -5,7 +5,7 @@ package software.amazon.cryptography.example.hierarchy;
 import javax.annotation.Nullable;
 import software.amazon.awssdk.services.dynamodb.DynamoDbClient;
 import software.amazon.cryptography.keystoreadmin.KeyStoreAdmin;
-import software.amazon.cryptography.keystoreadmin.model.KmsAesIdentifier;
+import software.amazon.cryptography.keystoreadmin.model.KmsSymmetricKeyArn;
 import software.amazon.cryptography.keystoreadmin.model.VersionKeyInput;
 
 /*
@@ -63,7 +63,7 @@ public class VersionKeyExample {
         // This is the KMS ARN that will be used to protect the Branch Key.
         // It is a required argument.
         // This ARN MUST match the ARN that protects the Branch Key.
-        .KmsArn(KmsAesIdentifier.builder().KmsKeyArn(kmsKeyArn).build())
+        .KmsArn(KmsSymmetricKeyArn.builder().KmsKeyArn(kmsKeyArn).build())
         // This the Identifier for the Branch Key that is being rotated/versioned.
         .Identifier(branchKeyId)
         .build()
