AwsCryptographicMaterialProviders/dafny/AwsCryptographyKeyStoreAdmin/Model/AwsCryptographyKeyStoreAdminTypes.dfy
@@ -22,7 +22,7 @@ module {:extern "software.amazon.cryptography.keystoreadmin.internaldafny.types"
     nameonly MutationToken: MutationToken ,
     nameonly PageSize: Option<int32> := Option.None ,
     nameonly Strategy: Option<KeyManagementStrategy> := Option.None ,
-    nameonly SystemKey: SystemKey
+    nameonly SystemKey: Option<SystemKey> := Option.None
   )
   datatype ApplyMutationOutput = | ApplyMutationOutput (
     nameonly MutationResult: ApplyMutationResult ,
@@ -34,7 +34,7 @@ module {:extern "software.amazon.cryptography.keystoreadmin.internaldafny.types"
   datatype CreateKeyInput = | CreateKeyInput (
     nameonly Identifier: Option<string> := Option.None ,
     nameonly EncryptionContext: Option<AwsCryptographyKeyStoreTypes.EncryptionContext> := Option.None ,
-    nameonly KmsArn: KmsAesIdentifier ,
+    nameonly KmsArn: KmsSymmetricKeyArn ,
     nameonly Strategy: Option<KeyManagementStrategy> := Option.None
   )
   datatype CreateKeyOutput = | CreateKeyOutput (
@@ -44,18 +44,18 @@ module {:extern "software.amazon.cryptography.keystoreadmin.internaldafny.types"
     nameonly Identifier: string
   )
   datatype DescribeMutationOutput = | DescribeMutationOutput (
-    nameonly Original: Option<MutableBranchKeyProperities> := Option.None ,
-    nameonly Terminal: Option<MutableBranchKeyProperities> := Option.None
+    nameonly MutationInFlight: MutationInFlight
   )
   datatype InitializeMutationFlag =
-    | Created(Created: string)
-    | Resumed(Resumed: string)
-    | ResumedWithoutIndex(ResumedWithoutIndex: string)
+    | Created
+    | Resumed
+    | ResumedWithoutIndex
   datatype InitializeMutationInput = | InitializeMutationInput (
     nameonly Identifier: string ,
     nameonly Mutations: Mutations ,
     nameonly Strategy: Option<KeyManagementStrategy> := Option.None ,
-    nameonly SystemKey: SystemKey
+    nameonly SystemKey: Option<SystemKey> := Option.None ,
+    nameonly DoNotVersion: Option<bool> := Option.None
   )
   datatype InitializeMutationOutput = | InitializeMutationOutput (
     nameonly MutationToken: MutationToken ,
@@ -185,14 +185,14 @@ module {:extern "software.amazon.cryptography.keystoreadmin.internaldafny.types"
     nameonly logicalKeyStoreName: string ,
     nameonly storage: AwsCryptographyKeyStoreTypes.Storage
   )
-  datatype KmsAes = | KmsAes (
-    nameonly KmsAesIdentifier: KmsAesIdentifier ,
+  datatype KmsSymmetricEncryption = | KmsSymmetricEncryption (
+    nameonly KmsArn: KmsSymmetricKeyArn ,
     nameonly AwsKms: AwsCryptographyKeyStoreTypes.AwsKms
   )
-  datatype KmsAesIdentifier =
+  datatype KmsSymmetricKeyArn =
     | KmsKeyArn(KmsKeyArn: string)
     | KmsMRKeyArn(KmsMRKeyArn: string)
-  datatype MutableBranchKeyProperities = | MutableBranchKeyProperities (
+  datatype MutableBranchKeyProperties = | MutableBranchKeyProperties (
     nameonly KmsArn: string ,
     nameonly CustomEncryptionContext: AwsCryptographyKeyStoreTypes.EncryptionContextString
   )
@@ -204,24 +204,39 @@ module {:extern "software.amazon.cryptography.keystoreadmin.internaldafny.types"
   datatype MutationComplete = | MutationComplete (
 
                               )
+  datatype MutationDescription = | MutationDescription (
+    nameonly MutationDetails: MutationDetails ,
+    nameonly MutationToken: MutationToken
+  )
+  datatype MutationDetails = | MutationDetails (
+    nameonly Original: MutableBranchKeyProperties ,
+    nameonly Terminal: MutableBranchKeyProperties ,
+    nameonly Input: Mutations ,
+    nameonly SystemKey: string ,
+    nameonly CreateTime: string ,
+    nameonly UUID: string
+  )
+  datatype MutationInFlight =
+    | Yes(Yes: MutationDescription)
+    | No(No: string)
   datatype Mutations = | Mutations (
     nameonly TerminalKmsArn: Option<string> := Option.None ,
     nameonly TerminalEncryptionContext: Option<AwsCryptographyKeyStoreTypes.EncryptionContextString> := Option.None
   )
   datatype MutationToken = | MutationToken (
     nameonly Identifier: string ,
-    nameonly UUID: Option<string> := Option.None ,
+    nameonly UUID: string ,
     nameonly CreateTime: string
   )
   datatype SystemKey =
-    | kmsAes(kmsAes: KmsAes)
+    | kmsSymmetricEncryption(kmsSymmetricEncryption: KmsSymmetricEncryption)
     | trustStorage(trustStorage: TrustStorage)
   datatype TrustStorage = | TrustStorage (
 
                           )
   datatype VersionKeyInput = | VersionKeyInput (
     nameonly Identifier: string ,
-    nameonly KmsArn: KmsAesIdentifier ,
+    nameonly KmsArn: KmsSymmetricKeyArn ,
     nameonly Strategy: Option<KeyManagementStrategy> := Option.None
   )
   datatype VersionKeyOutput = | VersionKeyOutput (
@@ -241,9 +256,6 @@ module {:extern "software.amazon.cryptography.keystoreadmin.internaldafny.types"
     | MutationInvalidException (
         nameonly message: string
       )
-    | MutationLockInvalidException (
-        nameonly message: string
-      )
     | MutationToException (
         nameonly message: string
       )
@@ -251,6 +263,9 @@ module {:extern "software.amazon.cryptography.keystoreadmin.internaldafny.types"
         nameonly message: string
       )
     | UnexpectedStateException (
+        nameonly message: string
+      )
+    | UnsupportedFeatureException (
         nameonly message: string
       )
       // Any dependent models are listed here
